DynamoDbEncryption/dafny/StructuredEncryption/src/Footer.dfy
@@ -140,16 +140,28 @@ module StructuredEncryptionFooter {
     }
   }
 
+  const ENCRYPTED : UTF8.ValidUTF8Bytes :=
+    var s := [0x45, 0x4e, 0x43, 0x52, 0x59, 0x50, 0x54, 0x45, 0x44];
+    assert s == UTF8.EncodeAscii("ENCRYPTED");
+    s
+
+  const PLAINTEXT : UTF8.ValidUTF8Bytes :=
+    var s := [0x50, 0x4c, 0x41, 0x49, 0x4e, 0x54, 0x45, 0x58, 0x54];
+    assert s == UTF8.EncodeAscii("PLAINTEXT");
+    s
+
+
+
   // Given a StructuredDataTerminal, return the canonical value for the type, for use in the footer checksum calculations
   function method GetCanonicalType(value : StructuredDataTerminal, isEncrypted : bool)
     : Result<Bytes, Error>
   {
     if isEncrypted then
       :- Need(2 <= |value.value| < UINT64_LIMIT, E("Bad length."));
-      Success(UInt64ToSeq((|value.value| - 2) as uint64) + UTF8.EncodeAscii("ENCRYPTED"))
+      Success(UInt64ToSeq((|value.value| - 2) as uint64) + ENCRYPTED)
     else
       :- Need(|value.value| < UINT64_LIMIT, E("Bad length."));
-      Success(UInt64ToSeq((|value.value|) as uint64) + UTF8.EncodeAscii("PLAINTEXT") + value.typeId)
+      Success(UInt64ToSeq((|value.value|) as uint64) + PLAINTEXT + value.typeId)
   }
 
   function method GetCanonicalEncryptedField(fieldName : CanonicalPath, value : StructuredDataTerminal)
@@ -169,14 +181,14 @@ module StructuredEncryptionFooter {
               && ret.value ==
                  fieldName
                  + UInt64ToSeq((|value.value| - 2) as uint64)
-                 + UTF8.EncodeAscii("ENCRYPTED")
+                 + ENCRYPTED
                  + value.value // this is 2 bytes of unencrypted type, followed by encrypted value
   {
     :- Need(2 <= |value.value| < UINT64_LIMIT, E("Bad length."));
     Success(
       fieldName
       + UInt64ToSeq((|value.value| - 2) as uint64)
-      + UTF8.EncodeAscii("ENCRYPTED")
+      + ENCRYPTED
       + value.value
     )
   }
@@ -198,7 +210,7 @@ module StructuredEncryptionFooter {
               && ret.value ==
                  fieldName
                  + UInt64ToSeq((|value.value|) as uint64)
-                 + UTF8.EncodeAscii("PLAINTEXT")
+                 + PLAINTEXT
                  + value.typeId
                  + value.value
   {
@@ -206,7 +218,7 @@ module StructuredEncryptionFooter {
     Success(
       fieldName
       + UInt64ToSeq((|value.value|) as uint64)
-      + UTF8.EncodeAscii("PLAINTEXT")
+      + PLAINTEXT
       + value.typeId
       + value.value
     )
